

A set of vectors $\{\bar{v}_1, \bar{v}_2, \dots, \bar{v}_n\}$ is said to form a basis for a vector space. IF:

- ① The vectors $\bar{v}_1, \bar{v}_2, \dots, \bar{v}_n$ span the vector space.
- ② The vectors $\bar{v}_1, \bar{v}_2, \dots, \bar{v}_n$ L. Ind.

For example: $\begin{bmatrix} 1 \\ 0 \\ 0 \end{bmatrix}, \begin{bmatrix} 0 \\ 1 \\ 0 \end{bmatrix}, \begin{bmatrix} 0 \\ 0 \\ 1 \end{bmatrix}$ are a basis of \mathbb{R}^3 .

Do the vectors: $\begin{bmatrix} 1 \\ 1 \\ 1 \end{bmatrix}, \begin{bmatrix} 0 \\ 1 \\ 0 \end{bmatrix}, \begin{bmatrix} 1 \\ 2 \\ 3 \end{bmatrix}$.

also form a basis for \mathbb{R}^3 ?

Independence?

$$\left[\begin{array}{ccc|c} 1 & 0 & 1 & 0 \\ 1 & 1 & 2 & 0 \\ 1 & 0 & 3 & 0 \end{array} \right] \sim \left[\begin{array}{ccc|c} 1 & 0 & 1 & 0 \\ 0 & 1 & 1 & 0 \\ 0 & 0 & 2 & 0 \end{array} \right] \sim \left[\begin{array}{ccc|c} 1 & 0 & 1 & 0 \\ 0 & 1 & 1 & 0 \\ 0 & 0 & 1 & 0 \end{array} \right]$$

$$\begin{array}{l} -1R_1 + R_2 \rightarrow R_2 \\ -1R_1 + R_3 \rightarrow R_3 \end{array}$$

$$\frac{1}{2}R_3 \rightarrow R_3$$

$$\begin{array}{l} -1R_3 + R_1 \rightarrow R_1 \\ -1R_3 + R_2 \rightarrow R_2 \end{array}$$

$$\sim \left[\begin{array}{ccc|c} 1 & 0 & 0 & 0 \\ 0 & 1 & 0 & 0 \\ 0 & 0 & 1 & 0 \end{array} \right]$$

$$\begin{array}{c} a_1 \ a_2 \ a_3 \\ \left[\begin{array}{ccc|c} 1 & 0 & 0 & 0 \\ 0 & 1 & 0 & 0 \\ 0 & 0 & 1 & 0 \end{array} \right] \end{array}$$

$\therefore a_1 = 0$
 $a_2 = 0$
 $a_3 = 0 \Rightarrow$ Trivial solution. \therefore L. Ind.

Span.

$$a_1 \begin{bmatrix} 1 \\ 1 \\ 1 \end{bmatrix} + a_2 \begin{bmatrix} 0 \\ 1 \\ 0 \end{bmatrix} + a_3 \begin{bmatrix} 1 \\ 2 \\ 3 \end{bmatrix} = \begin{bmatrix} x \\ y \\ z \end{bmatrix}$$

$$\begin{aligned} 1a_1 + 1a_3 &= x \\ 1a_1 + 1a_2 + 2a_3 &= y \\ 1a_1 + 3a_3 &= z \end{aligned}$$

Solve a_1, a_2, a_3 .

Use substitution.

$$a_1 + a_3 = x \rightarrow a_1 = x - a_3$$

$$a_1 + 3a_3 = z$$

$$x - a_3 + 3a_3 = z$$

$$x + 2a_3 = z$$

$$a_3 = \frac{z - x}{2}$$

$$a_1 = x - \frac{z - x}{2}$$

$$a_1 = \frac{3}{2}x - \frac{z}{2}$$

$$a_1 + a_2 + 2a_3 = y$$

$$\frac{3}{2}x - \frac{1}{2}z + a_2 + 2 \cdot \frac{z - x}{2} = y$$

$$\frac{3}{2}x - \frac{1}{2}z + z - x + a_2 = y$$

$$\frac{1}{2}x + \frac{1}{2}z + a_2 = y$$

$$a_2 = y - \frac{1}{2}x - \frac{1}{2}z$$

$$2x + 2z = 4x - y$$

$$a_2 = y - \frac{1}{2}x - \frac{1}{2}z$$

$$a_2 = -\frac{1}{2}x + y - \frac{1}{2}z$$

So they are form a spanning set.